src/examples/simple_base.v
@@ -47,7 +47,8 @@ Section simple_increment.
   Proof.
     iIntros (Φ) "#val Post".
     rewrite /alloc_load.
-    wp_alloc ℓ as "pts".
+    wp_apply (wp_alloc with "[$]"). iIntros (ℓ ?) "(_ & _ & _ & pts)".
+    wp_pures.
     wp_pures.
     iApply (wp_load with "[$pts $val]").
     iNext. iIntros (t v msg) "(pts & %look & %msgEq & gt)".
